It is LL(1) as:
\begin{center}
    $la(S \rightarrow R) = \{(, a, b\}$ \\
    $la(R \rightarrow TR') = \{(, a, b\}$ \\
    \begin{equation}
      \cap = \varnothing
      \begin{cases}
        la(R' \rightarrow +TR') = \{+\$ \\
        la(R' \rightarrow TR') = \{(, a, b\} \\
        la(R' \rightarrow \cdot TR') = \{\cdot\} \\
        la(R' \rightarrow \varepsilon) = \{ \varepsilon, )\} \\
    \end{cases}  
    \end{equation}
    \begin{equation}
        \cap = \varnothing
        \begin{cases}
            la(T \rightarrow (R)) = \{(\} \\
            la(T \rightarrow a) = \{a\} \\
            la(T \rightarrow b) = \{b\} \\  
        \end{cases}
    \end{equation}
\end{center}


